wip

dafny/prime.dfy
@@ -18,20 +18,28 @@ module Prime {
     }
 
     function method isPrime(prime: nat): bool
+        ensures prime < 2 ==> isPrime(prime) == false;
     {
         if prime < 2 then false
         else isPrimeLoop(prime, prime - 1)
     }
 
+
+    function method allPrimesAreInTheList(list: seq<nat>):bool
+    {
+        |list| > 0 ==> 
+            forall v :: 2 <= v <= List.max(list) ==> 
+            ( 
+                isPrime(v) ==> exists k  :: 0 <= k < |list| && list[k] == v
+            )
+    }
+
     function method isPrimeSequence(list: seq<nat>): bool        
     {
         var allElementsArePrimes := forall k :: 0 <= k < |list| ==> isPrime(list[k]);
-        var allPrimesAreInTheList := |list| > 0 ==> 
-            forall v :: 2 <= v <= List.max(list) ==> ( 
-                isPrime(v) ==> exists k  :: 0 <= k < |list| && list[k] == v
-            );
-        var isSorted := List.sorted(list);
+        var isSorted := List.sortedDesc(list);
         var isNonZero := List.nonZero(list);
+        var allPrimesAreInTheList := allPrimesAreInTheList(list);
 
         if !isSorted then false
         else if !isNonZero then false
@@ -46,6 +54,7 @@ module Prime {
         ensures value >= 2 && isPrime(value) ==> |getPrimeSequenceUntil(value)| > 0;
         ensures value >= 2 && isPrime(value) ==> getPrimeSequenceUntil(value)[0] == value;
         decreases value;
+        ensures forall k :: 0 <= k < |getPrimeSequenceUntil(value)| ==> getPrimeSequenceUntil(value)[k] <= value;
     {
         var prev := if value < 2 then [] else getPrimeSequenceUntil(value - 1);
         var primeSequence := if value < 2 then []
@@ -62,7 +71,17 @@ module Prime {
 
     lemma getPrimeSequenceUntilValueIsPrimeSequence(value: nat, primeSequence: seq<nat>)
         requires primeSequence == getPrimeSequenceUntil(value);
-        // ensures isPrimeSequence(primeSequence);
+        ensures |primeSequence| > 1 ==> primeSequence[0] > primeSequence[1];
+        ensures List.sortedDesc(primeSequence);
+        ensures List.nonZero(primeSequence);
+        ensures allPrimesAreInTheList(primeSequence);
+        ensures isPrime(value) ==> |primeSequence| > 0;
+        ensures isPrime(value) ==> primeSequence[0] == value;
+        ensures value < 2 ==> primeSequence == [];
+        ensures value < 2 ==> isPrime(value) == false;
+        ensures isPrime(value) ==> primeSequence[0] == value;
+        ensures isPrime(value) ==> primeSequence[1..] == getPrimeSequenceUntil(value - 1);
+        ensures !isPrime(value) ==> primeSequence == getPrimeSequenceUntil(value - 1);
     {
         assert forall v :: 0 <= v < 2 ==> isPrime(v) == false;
         if (value < 2) {
@@ -71,32 +90,13 @@ module Prime {
             if (isPrime(value)) {
                 assert primeSequence[0] == value;
                 assert primeSequence[1..] == getPrimeSequenceUntil(value - 1);
+                getPrimeSequenceUntilValueIsPrimeSequence(value -1, primeSequence[1..]);
             } else {
                 assert primeSequence == getPrimeSequenceUntil(value - 1);
-            }
-            if (isPrime(value) && isPrime(value - 1))
-            {
-                assert primeSequence[0] == value;
-                assert primeSequence[1] == value - 1;
-                assert primeSequence[1] < primeSequence[0];
-            }
-            if (isPrime(value) && !isPrime(value - 1))
-            {
-                assert primeSequence[0] == value;
-                assert primeSequence[1..] == getPrimeSequenceUntil(value - 2);
-                getPrimeSequenceUntilValueIsPrimeSequence(value - 2, primeSequence[1..]);
-            }
-            if (!isPrime(value) && isPrime(value - 1))
-            {
-                assert primeSequence == getPrimeSequenceUntil(value - 1);
-                getPrimeSequenceUntilValueIsPrimeSequence(value - 1, primeSequence);
-            }
-            if (!isPrime(value) && !isPrime(value - 1))
-            {
-                assert primeSequence == getPrimeSequenceUntil(value - 2);
-                getPrimeSequenceUntilValueIsPrimeSequence(value - 2, primeSequence);
-            }
+                getPrimeSequenceUntilValueIsPrimeSequence(value -1, primeSequence);
+            } 
             assert |primeSequence| > 1 ==> primeSequence[0] > primeSequence[1];
+            assert forall k : nat :: 1 <= k < |primeSequence| ==> primeSequence[k] < primeSequence[k-1];
         }
     }
 
